ROOT
@@ -1,16 +1,23 @@
-session "Congruence_Closure" = HOL +
+session "Union_Find_Explain" in Union_Find_Explain = HOL +
   sessions
     "HOL-Library"
     Separation_Logic_Imperative_HOL
-  directories
-    Union_Find_Explain
-    Congruence_CLosure_Explain
   theories
     Explain
     Path
     Proofs
     Explain_Proofs
     Explain_Proofs2
+
+session "Congruence_Closure" in Congruence_Closure_Explain = HOL +
+  sessions
+    "HOL-Library"
+    Separation_Logic_Imperative_HOL
+    Union_Find_Explain
+  theories
     Congruence_Closure
+    CC_Proofs
+    CC_Abstraction
+    Congruence_Closure_Proofs
     
 
